feat: Zen.Sha3.Extracted.hashWith

fstar/Zen.Sha3.Extracted.fst
@@ -2,6 +2,7 @@ module Zen.Sha3.Extracted
 
 open Zen.Base
 open Zen.Cost
+open Zen.Types
 
 module Sha3 = Zen.Sha3.Realized
 module PK = Zen.PublicKey
@@ -11,7 +12,7 @@ let updateCPK (parity, h) s =
   ret s
   >>= Sha3.updateByte parity
   >>= Sha3.updateHash h
-  |> Zen.Cost.inc 7
+  |> inc 7
 
 val updateListWith (#a : Type) (#n : nat) :
     (a -> Sha3.t -> Sha3.t `cost` n)
@@ -20,4 +21,14 @@ val updateListWith (#a : Type) (#n : nat) :
     -> Sha3.t `cost` (length ls * (n + 4) + 8)
 let updateListWith #_ #_ upd ls sha3 =
   Zen.List.foldT (flip upd) sha3 ls
-  |> Zen.Cost.inc 4
+  |> inc 4
+
+val hashWith (#a : Type) (#n : nat) :
+    (a -> Sha3.t -> Sha3.t `cost` n)
+    -> a
+    -> hash `cost` (n + 26)
+let hashWith #_ #_ upd x =
+  ret Sha3.empty
+  >>= upd x
+  >>= Sha3.finalize
+  |> inc 6
